Low-level specs for config service

src/program_proof/simplepb/config_proof.v
@@ -5,11 +5,74 @@ From iris.algebra Require Import dfrac_agree mono_list.
 
 Section config_proof.
 
-Class configG Σ := {
-    config_epochG :> mono_natG Σ ;
-    config_configG :> inG Σ (gmapR u64 (dfrac_agreeR (leibnizO (option (list u64))))) ;
+Record config_names :=
+{
+  epoch_gn:gname ;
+  config_val_gn:gname;
 }.
 
-Context
+Class configG Σ := {
+    config_epochG :> mono_natG Σ ;
+    config_configG :> inG Σ (dfrac_agreeR (leibnizO (list u64)));
+}.
+
+Implicit Type γ : config_names.
+
+Context `{!heapGS Σ}.
+Context `{!configG Σ}.
+
+Definition own_epoch γ (epoch:u64) : iProp Σ :=
+  mono_nat_auth_own γ.(epoch_gn) (1/2) (int.nat epoch).
+Definition is_epoch_lb γ (epoch:u64) : iProp Σ :=
+  mono_nat_lb_own γ.(epoch_gn) (int.nat epoch).
+
+Definition own_config γ (conf:list u64) : iProp Σ :=
+  own γ.(config_val_gn) (to_dfrac_agree (DfracOwn (1/2)) (conf: (leibnizO _)))
+.
+
+Definition is_host (configHost:u64) γ : iProp Σ := True.
+
+Definition is_Clerk (ck:loc) γ : iProp Σ := True.
+
+Lemma wp_MakeClerk configHost γ:
+  {{{
+      is_host configHost γ
+  }}}
+    config.MakeClerk #configHost
+  {{{
+      ck, RET #ck; is_Clerk ck γ
+  }}}
+.
+Proof.
+Admitted.
+
+Lemma wp_Clerk__GetEpochAndConfig (ck:loc) γ Φ :
+  is_Clerk ck γ -∗
+  □ (|={⊤,∅}=> ∃ epoch conf, own_epoch γ epoch ∗
+                                    own_config γ conf ∗
+    (own_epoch γ (word.add epoch 1) ={∅,⊤}=∗
+      (∀ oldServers_sl, Φ (#(LitInt (word.add epoch 1)), slice_val oldServers_sl)%V)
+                                )
+  ) -∗
+  WP config.Clerk__GetEpochAndConfig #ck {{ Φ }}
+.
+Proof.
+Admitted.
+
+Lemma wp_Clerk__WriteConfig (ck:loc) new_conf new_conf_sl epoch γ Φ :
+  is_Clerk ck γ -∗
+  is_slice new_conf_sl uint64T 1 new_conf ∗
+  is_epoch_lb γ epoch -∗
+  □ (|={⊤,∅}=> ∃ latest_epoch, own_epoch γ latest_epoch ∗
+      if (decide (latest_epoch = epoch)) then
+        ∃ conf, own_config γ conf ∗ (own_config γ new_conf -∗ own_epoch γ epoch ={∅,⊤}=∗ Φ #0)
+      else
+        (own_epoch γ latest_epoch ={∅,⊤}=∗ (∀ (err:u64), ⌜err ≠ 0⌝ → Φ #err))
+  ) -∗
+  WP config.Clerk__WriteConfig #ck #epoch
+  {{ Φ }}
+.
+Proof.
+Admitted.
 
 End config_proof.
